#
# Copyright (c) 2011 Joerg Ehrichs <Joerg.Ehrichs@gmx.de>
#
# All rights reserved, licensed under either CC-BY or BSD.
#
# You are free:
#  * to Share - to copy, distribute and transmit the work
#  * to Remix - to adapt the work
# Under the following conditions:
#  * Attribution - You must attribute the work in the manner specified by the author
#    or licensor (but not in any way that suggests that they endorse you or your use 
#    of the work).
#
# Redistribution and use in source and binary forms, with or without modification, 
# are permitted provided that the following conditions are met:
#  * Redistributions of source code must retain the above copyright notice, this 
#    list of conditions and the following disclaimer.
#  * Redistributions in binary form must reproduce the above copyright notice, this 
#    list of conditions and the following disclaimer in the documentation and/or 
#    other materials provided with the distribution.
#  * Neither the names of the authors nor the names of contributors may
#    be used to endorse or promote products derived from this ontology without 
#    specific prior written permission.
#
# THIS ONTOLOGY IS PROVIDED BY THE AUTHOR ``AS IS'' AND ANY EXPRESS OR
# IMPLIED WARRANTIES, INCLUDING, BUT NOT LIMITED TO, THE IMPLIED WARRANTIES
# OF MERCHANTABILITY AND FITNESS FOR A PARTICULAR PURPOSE ARE DISCLAIMED.
# IN NO EVENT SHALL THE AUTHOR BE LIABLE FOR ANY DIRECT, INDIRECT,
# INCIDENTAL, SPECIAL, EXEMPLARY, OR CONSEQUENTIAL DAMAGES (INCLUDING, BUT
# NOT LIMITED TO, PROCUREMENT OF SUBSTITUTE GOODS OR SERVICES; LOSS OF USE,
# DATA, OR PROFITS; OR BUSINESS INTERRUPTION) HOWEVER CAUSED AND ON ANY
# THEORY OF LIABILITY, WHETHER IN CONTRACT, STRICT LIABILITY, OR TORT
# (INCLUDING NEGLIGENCE OR OTHERWISE) ARISING IN ANY WAY OUT OF THE USE OF
# THIS ONTOLOGY, EVEN IF ADVISED OF THE POSSIBILITY OF SUCH DAMAGE.
#

@prefix nbib:    <http://www.example.com/nbib#> .
@prefix rdfs:    <http://www.w3.org/2000/01/rdf-schema#> .
@prefix rdf:     <http://www.w3.org/1999/02/22-rdf-syntax-ns#> .
@prefix dc:      <http://purl.org/dc/elements/1.1/> .
@prefix xsd:     <http://www.w3.org/2001/XMLSchema#> .
@prefix nrl:     <http://www.semanticdesktop.org/ontologies/2007/08/15/nrl#> .
@prefix nie:     <http://www.semanticdesktop.org/ontologies/2007/01/19/nie#> .
@prefix nfo:     <http://www.semanticdesktop.org/ontologies/2007/03/22/nfo#> .
@prefix nco:     <http://www.semanticdesktop.org/ontologies/2007/03/22/nco#> .
@prefix nao:     <http://www.semanticdesktop.org/ontologies/2007/08/15/nao#> .
@prefix ncal:    <http://www.semanticdesktop.org/ontologies/2007/04/02/ncal#> .
@prefix pimo:    <http://www.semanticdesktop.org/ontologies/2007/11/01/pimo#> .

nbib: {
    nbib:Reference
          a       rdfs:Class ;
          rdfs:comment "A bibliographic reference" ;
          rdfs:label "Bibliographic Reference" ;
          rdfs:subClassOf nie:InformationElement .

####################################################################
#
# Resource Types
# these can be translated back into BibTeX entries

    nbib:Publication
          a       rdfs:Class ;
          rdfs:comment "A bibliographic reference resource type (article, book, paper and such)" ;
          rdfs:label "Bibliographic Publication" ;
          rdfs:subClassOf nie:InformationElement .

    nbib:Article
          a       rdfs:Class ;
          rdfs:comment "An article from a journal or magazine." ;
          rdfs:label "Article" ;
          rdfs:subClassOf nbib:Publication .

    nbib:BachelorThesis
          a       rdfs:Class ;
          rdfs:comment "A Bachelor thesis." ;
          rdfs:label "Bachelorthesis" ;
          rdfs:subClassOf nbib:Thesis .

    nbib:Book
          a       rdfs:Class ;
          rdfs:comment "A book with an explicit publisher." ;
          rdfs:label "Book" ;
          rdfs:subClassOf nbib:Publication .

    nbib:Booklet
          a       rdfs:Class ;
          rdfs:comment "A work that is printed and bound, but without a named publisher or sponsoring institution." ;
          rdfs:label "Booklet" ;
          rdfs:subClassOf nbib:Publication .

    nbib:Collection
          a       rdfs:Class ;
          rdfs:comment "A collection of different publications." ;
          rdfs:label "Collection" ;
          rdfs:subClassOf nbib:Publication .

    nbib:Dictionary
          a       rdfs:Class ;
          rdfs:comment "A dictionary" ;
          rdfs:label "Dictionary" ;
          rdfs:subClassOf nbib:Book .

    nbib:Encyclopedia
          a       rdfs:Class ;
          rdfs:comment "A encyclopedia" ;
          rdfs:label "Encyclopedia" ;
          rdfs:subClassOf nbib:Collection .

    nbib:Electronic
          a       rdfs:Class ;
          rdfs:comment "An electronic publication (for example website or presentations)" ;
          rdfs:label "Electronic source" ;
          rdfs:subClassOf nbib:Publication .

    nbib:Map
          a       rdfs:Class ;
          rdfs:comment "A map with geographical data" ;
          rdfs:label "Map" ;
          rdfs:subClassOf nbib:Publication .

    nbib:ForumPost
          a       rdfs:Class ;
          rdfs:comment "Reference the post in a forum or other electronic list" ;
          rdfs:label "Forum Post" ;
          rdfs:subClassOf nbib:Article .

    nbib:Forum
          a       rdfs:Class ;
          rdfs:comment "Reference the forum in which several ForumPost can be found" ;
          rdfs:label "Forum" ;
          rdfs:subClassOf nbib:Collection .

    nbib:BlogPost
          a       rdfs:Class ;
          rdfs:comment "Reference the post in a web log (blog)" ;
          rdfs:label "Blog Post" ;
          rdfs:subClassOf nbib:Article .

    nbib:Blog
          a       rdfs:Class ;
          rdfs:comment "Reference the blog in which several BlogPost can be found" ;
          rdfs:label "Blog" ;
          rdfs:subClassOf nbib:Collection .

    nbib:Webpage
          a       rdfs:Class ;
          rdfs:comment "Reference a webpage in general (only one site of the complete Website)" ;
          rdfs:label "Webpage" ;
          rdfs:subClassOf nbib:Article .

    nbib:Website
          a       rdfs:Class ;
          rdfs:comment "Reference the complete website in which several webpages can be found" ;
          rdfs:label "Website" ;
          rdfs:subClassOf nbib:Collection .

    nbib:LegalDocument
          a       rdfs:Class ;
          rdfs:comment "A legal document; for example, a court decision, a brief, and so forth." ;
          rdfs:label "Legal Document" ;
          rdfs:subClassOf nbib:Publication .

    nbib:Legislation
          a       rdfs:Class ;
          rdfs:comment "A legal document proposing or enacting a law or a group of laws." ;
          rdfs:label "Legislation" ;
          rdfs:subClassOf nbib:LegalDocument .

    nbib:Bill
          a       rdfs:Class ;
          rdfs:comment "Draft legislation presented for discussion to a legal body." ;
          rdfs:label "Bill" ;
          rdfs:subClassOf nbib:Legislation .

    nbib:Statute
          a       rdfs:Class ;
          rdfs:comment "A bill enacted into law." ;
          rdfs:label "Statute" ;
          rdfs:subClassOf nbib:Legislation .

    nbib:LegalCaseDocument
          a       rdfs:Class ;
          rdfs:comment "A document accompanying a legal case." ;
          rdfs:label "LegalCaseDocument" ;
          rdfs:subClassOf nbib:LegalDocument .

    nbib:Brief
          a       rdfs:Class ;
          rdfs:comment "A written argument submitted to a court." ;
          rdfs:label "Brief" ;
          rdfs:subClassOf nbib:LegalCaseDocument .

    nbib:Decision
          a       rdfs:Class ;
          rdfs:comment "A document containing an authoritative determination (as a decree or judgment) made after consideration of facts or law." ;
          rdfs:label "Decision" ;
          rdfs:subClassOf nbib:LegalCaseDocument .

    nbib:Manual
          a       rdfs:Class ;
          rdfs:comment "Technical documentation." ;
          rdfs:label "Manual" ;
          rdfs:subClassOf nbib:Publication .

    nbib:MastersThesis
          a       rdfs:Class ;
          rdfs:comment "A Master's thesis." ;
          rdfs:label "Mastersthesis" ;
          rdfs:subClassOf nbib:Thesis .

    nbib:PhdThesis
          a       rdfs:Class ;
          rdfs:comment "A PhD thesis." ;
          rdfs:label "Phdthesis" ;
          rdfs:subClassOf nbib:Thesis .

    nbib:Presentation
          a       rdfs:Class ;
          rdfs:comment "Slides for a presentation" ;
          rdfs:label "Presentation" ;
          rdfs:subClassOf nbib:Publication .

    nbib:Proceedings
          a       rdfs:Class ;
          rdfs:comment "The proceedings of a conference." ;
          rdfs:label "Proceedings" ;
          rdfs:subClassOf nbib:Collection .

    nbib:Report
          a       rdfs:Class ;
          rdfs:comment "A document describing an account or statement describing in detail an event, situation, or the like, usually as the result of observation, inquiry, etc.." ;
          rdfs:label "Report" ;
          rdfs:subClassOf nbib:Publication .

    nbib:Script
          a       rdfs:Class ;
          rdfs:comment "The script for something (a lecture for ecxample)" ;
          rdfs:label "Script" ;
          rdfs:subClassOf nbib:Publication .

    nbib:Standard
          a       rdfs:Class ;
          rdfs:comment "A document describing a standard" ;
          rdfs:label "Standard" ;
          rdfs:subClassOf nbib:Publication .

    nbib:Techreport
          a       rdfs:Class ;
          rdfs:comment "A report published by a school or other institution, usually numbered within a series." ;
          rdfs:label "Techreport" ;
          rdfs:subClassOf nbib:Report .

    nbib:Thesis
          a       rdfs:Class ;
          rdfs:comment "A general thesis." ;
          rdfs:label "Thesis" ;
          rdfs:subClassOf nbib:Publication .

    nbib:Unpublished
          a       rdfs:Class ;
          rdfs:comment "A document having an author and title, but not formally published." ;
          rdfs:label "Unpublished" ;
          rdfs:subClassOf nbib:Publication .

    nbib:Patent
          a       rdfs:Class ;
          rdfs:comment "A patent." ;
          rdfs:label "Patent" ;
          rdfs:subClassOf nbib:Publication .

####################################################################
#
# Helper classes

    nbib:DocumentPart
          a       rdfs:Class ;
          rdfs:comment "a part of an document, mostly Chapters but alsow quotes etc. These don't have to be available as real file extracts but can also be linked to a real file, if available" ;
          rdfs:label "Document Part" ;
          rdfs:subClassOf nie:InformationElement .

    nbib:Chapter
          a       rdfs:Class ;
          rdfs:comment "A chapter of a publication." ;
          rdfs:label "Chapter" ;
          rdfs:subClassOf nbib:DocumentPart .

    nbib:Quote
          a       rdfs:Class ;
          rdfs:comment "A quote in a document" ;
          rdfs:label "Quote" ;
          rdfs:subClassOf nbib:DocumentPart .

    nbib:JournalIssue
          a       rdfs:Class ;
          rdfs:comment "A journal issue for serious, scholarly publications" ;
          rdfs:label "JournalIssue" ;
          rdfs:subClassOf nbib:Collection .

    nbib:MagazinIssue
          a       rdfs:Class ;
          rdfs:comment "A periodical of magazine Articles. A magazine is a publication that is issued periodically, usually bound in a paper cover, and typically contains essays, stories, poems, etc., by many writers, and often photographs and drawings, frequently specializing in a particular subject or area, as hobbies, news, or sports." ;
          rdfs:label "MagazinIssue" ;
          rdfs:subClassOf nbib:Collection .

    nbib:Series
          a       rdfs:Class ;
          rdfs:comment "Superclass to represent a series of some published data. (Book Series, Journal with several issues etc)" ;
          rdfs:label "Series" ;
          rdfs:subClassOf nie:InformationElement .

    nbib:BookSeries
          a       rdfs:Class ;
          rdfs:comment "The series of a book." ;
          rdfs:label "BookSeries" ;
          rdfs:subClassOf nbib:Series .

    nbib:CodeOfLaw
          a       rdfs:Class ;
          rdfs:comment "A collection of statutes." ;
          rdfs:label "CodeOfLaw" ;
          rdfs:subClassOf nbib:Collection .

    nbib:CourtReporter
          a       rdfs:Class ;
          rdfs:comment "A collection of legal cases." ;
          rdfs:label "Court Reporter" ;
          rdfs:subClassOf nbib:Collection .

    nbib:Journal
          a       rdfs:Class ;
          rdfs:comment "A Journal which publish single journal issues." ;
          rdfs:label "Journal" ;
          rdfs:subClassOf nbib:Series .

    nbib:Magazin
          a       rdfs:Class ;
          rdfs:comment "A Magazin which publish several MagazinIssue containing several articles" ;
          rdfs:label "Magazin" ;
          rdfs:subClassOf nbib:Series .

    nbib:Newspaper
          a       rdfs:Class ;
          rdfs:comment "A Newspaper which publish several NewspaperIssue containing several articles" ;
          rdfs:label "Newspaper" ;
          rdfs:subClassOf nbib:Series .

    nbib:NewspaperIssue
          a       rdfs:Class ;
          rdfs:comment "A single issue of a published Newspaper" ;
          rdfs:label "NewspaperIssue" ;
          rdfs:subClassOf nbib:Collection .

####################################################################
#
# To express the limited set of document/publication values for the status
# modelled after ncal:EventStatus idea with respect to bibo:DocumentStatus

    nbib:DocumentStatus
          a       rdfs:Class ;
          rdfs:comment "The status of the publication of a document." ;
          rdfs:label "DocumentStatus" ;
          rdfs:subClassOf rdfs:Resource .

    nbib:accepted
          a       nbib:DocumentStatus ;
          rdfs:comment "Accepted for publication after peer reviewing." ;
          rdfs:label "accepted" .

    nbib:draft
          a       nbib:DocumentStatus ;
          rdfs:comment "Document drafted." ;
          rdfs:label "draft" .

    nbib:forthcoming
          a       nbib:DocumentStatus ;
          rdfs:comment "Document to be published." ;
          rdfs:label "forthcoming" .

    nbib:legal
          a       nbib:DocumentStatus ;
          rdfs:comment "Legal document." ;
          rdfs:label "legal" .

    nbib:nonPeerReviewed
          a       nbib:DocumentStatus ;
          rdfs:comment "A document that is not peer reviewed." ;
          rdfs:label "non peer reviewed" .

    nbib:peerReviewed
          a       nbib:DocumentStatus ;
          rdfs:comment "The process by which articles are chosen to be included in a refereed journal. An editorial board consisting of experts in the same field as the author review the article and decide if it is authoritative enough for publication." ;
          rdfs:label "peer reviewed" .

    nbib:published
          a       nbib:DocumentStatus ;
          rdfs:comment "Published document." ;
          rdfs:label "published" .

    nbib:rejected
          a       nbib:DocumentStatus ;
          rdfs:comment "Rejected for publication after peer reviewing." ;
          rdfs:label "rejected" .

    nbib:unpublished
          a       nbib:DocumentStatus ;
          rdfs:comment "Unpublished document." ;
          rdfs:label "unpublished" .

    nbib:documentStatus
          a       rdf:Property ;
          rdfs:comment "The status of the publication of a document." ;
          rdfs:domain nbib:Publication ;
          rdfs:label "document status" ;
          rdfs:range nbib:DocumentStatus ;
          nrl:maxCardinality 1 .

####################################################################
#
# Properties

   nbib:affirmedBy
          a       rdf:Property ;
          rdfs:domain nbib:Decision ;
          rdfs:comment "A legal decision that affirms a ruling." ;
          rdfs:label "affirmedBy" ;
          rdfs:range nbib:Decision .

    nbib:translator
          a       rdf:Property ;
          rdfs:domain nbib:Publication ;
          rdfs:comment "The translator of a Publication" ;
          rdfs:label "translator" ;
          rdfs:range nco:Contact .

    nbib:contributor
          a       rdf:Property ;
          rdfs:domain nbib:Publication ;
          rdfs:comment "The contributor of a Publication" ;
          rdfs:label "contributor" ;
          rdfs:range nco:Contact .

    nbib:attorneyAgent
          a       rdf:Property ;
          rdfs:domain nbib:Patent ;
          rdfs:comment "A attorney agent related to a patent" ;
          rdfs:label "Attorney Agent" ;
          rdfs:range nco:Contact .

    nbib:counsel
          a       rdf:Property ;
          rdfs:domain nbib:LegalDocument ;
          rdfs:comment "The counsel related to a Legal document" ;
          rdfs:label "Counsel" ;
          rdfs:range nco:Contact .

    nbib:coSponsor
          a       rdf:Property ;
          rdfs:domain nbib:Legislation ;
          rdfs:comment "The co-sponsor [of a bill]" ;
          rdfs:label "Co-Sponsor" ;
          rdfs:range nco:Contact .

    nbib:reviewedAuthor
          a       rdf:Property ;
          rdfs:domain nbib:Publication ;
          rdfs:comment "The person who reviewed a Publication" ;
          rdfs:label "Reviewed Author" ;
          rdfs:range nco:Contact .

    nbib:commenter
          a       rdf:Property ;
          rdfs:domain nbib:Publication ;
          rdfs:comment "The commenter of a Publication. Mostly used for Blogs, Forum posts" ;
          rdfs:label "Commenter" ;
          rdfs:range nco:Contact .

    nbib:assignee
          a       rdf:Property ;
          rdfs:domain nbib:Patent ;
          rdfs:comment "The assignee of an patent" ;
          rdfs:label "assignee" ;
          rdfs:range nco:Contact .

   nbib:publishedAs
         a       rdf:Property ;
         rdfs:domain nfo:Document ;
         rdfs:comment "Links a document to its publication information." ;
         rdfs:label "publishedAs" ;
         rdfs:range nbib:Publication .

   nbib:isPublicationOf
         a       rdf:Property ;
         rdfs:domain nbib:Publication ;
         rdfs:comment "Links a publication to its document." ;
         rdfs:label "isPublicationOf" ;
         rdfs:range nfo:Document .

   nbib:courtReporter
         a       rdf:Property ;
         rdfs:domain nbib:LegalCaseDocument ;
         rdfs:comment "Links case document to the collection of legal cases it belongs to." ;
         rdfs:label "courtReporter" ;
         rdfs:range nbib:CourtReporter ;
         nrl:inverseProperty nbib:legalCase ;
          nrl:maxCardinality 1 .

   nbib:legalCase
         a       rdf:Property ;
         rdfs:domain nbib:CourtReporter ;
         rdfs:comment "Backlinks all legal cases from the court reporter it is from" ;
         rdfs:label "courtReporter" ;
         rdfs:range nbib:LegalCaseDocument ;
         nrl:inverseProperty nbib:courtReporter .

    nbib:citeKey
          a       rdf:Property ;
          rdfs:domain nbib:Reference ;
          rdfs:comment "Used to identify the reference." ;
          rdfs:label "CiteKey" ;
          rdfs:subPropertyOf nie:identifier ;
          rdfs:range xsd:string ;
          nrl:cardinality 1 ;
          nrl:maxCardinality 1 .

    nbib:chapterNumber
          a       rdf:Property ;
          rdfs:domain nbib:Chapter ;
          rdfs:comment "The number of the Chapter for example 1.2, II etc" ;
          rdfs:label "chapterNumber" ;
          rdfs:range xsd:string ;
          nrl:maxCardinality 1 .

    nbib:codeOfLaw
          a       rdf:Property ;
          rdfs:domain nbib:Legislation ;
          rdfs:comment "The code of law the legislation is contained in" ;
          rdfs:label "Code of Law" ;
          rdfs:range nbib:CodeOfLaw ;
          nrl:maxCardinality 1 .

    nbib:legislation
          a       rdf:Property ;
          rdfs:domain nbib:CodeOfLaw ;
          rdfs:comment "links to a legislation (Bill, Statute) in a Code of Law" ;
          rdfs:label "Legislation" ;
          rdfs:range nbib:Legislation .

    nbib:codeNumber
          a       rdf:Property ;
          rdfs:domain nbib:CodeOfLaw ;
          rdfs:comment "The code number of an CodeOfLaw" ;
          rdfs:label "CodeOfLaw number" ;
          rdfs:range xsd:string ;
          nrl:maxCardinality 1 .

    nie:abstract
          a       rdf:Property ;
          rdfs:domain nie:InformationElement ;
          rdfs:comment "An abstract of the work." ;
          rdfs:label "Abstract" ;
          rdfs:range xsd:string ;
          rdfs:subPropertyOf nao:description ;
          nrl:maxCardinality 1 .

    nfo:doi
          a       rdf:Property ;
          rdfs:domain nie:InformationElement ;
          rdfs:comment "The Digital object identifier. see http://www.doi.org/ for more information" ;
          rdfs:label "DOI" ;
          rdfs:range xsd:string ;
          rdfs:subPropertyOf nao:identifier ;
          nrl:maxCardinality 1 .

    nbib:edition
          a       rdf:Property ;
          rdfs:domain nbib:Publication ;
          rdfs:comment "The edition of a book, long form (such as 'first' or 'second')." ;
          rdfs:label "Edition" ;
          rdfs:range xsd:string ;
          nrl:maxCardinality 1 .

    nco:editor
          a       rdf:Property ;
          rdfs:domain nie:InformationElement ;
          rdfs:comment "The name(s) of the editor(s)." ;
          rdfs:label "Editor" ;
          rdfs:range nco:Contact .

    nbib:eprint
          a       rdf:Property ;
          rdfs:domain nbib:Publication ;
          rdfs:comment "A specification of an electronic publication, often a preprint or a technical report." ;
          rdfs:label "Eprint" ;
          rdfs:range xsd:string ;
          rdfs:subPropertyOf nao:identifier ;
          nrl:maxCardinality 1 .

    nbib:archive
          a       rdf:Property ;
          rdfs:domain nbib:Publication ;
          rdfs:comment "The archive where the publication can be found, see also nbib::archivelocation" ;
          rdfs:label "Archive" ;
          rdfs:range xsd:string ;
          nrl:maxCardinality 1 .

    nbib:archiveLocation
          a       rdf:Property ;
          rdfs:domain nbib:Publication ;
          rdfs:comment "The location where the publication can be found in the archive specified via nbib::archive" ;
          rdfs:label "Archive Location" ;
          rdfs:range xsd:string ;
          nrl:maxCardinality 1 .

    nbib:libraryCatalog
          a       rdf:Property ;
          rdfs:domain nbib:Publication ;
          rdfs:comment "The library catalog information where the publication can be found" ;
          rdfs:label "Library Catalog" ;
          rdfs:range xsd:string ;
          nrl:maxCardinality 1 .

    nbib:history
          a       rdf:Property ;
          rdfs:domain nbib:LegalDocument ;
          rdfs:comment "The history of a legal document" ;
          rdfs:label "History" ;
          rdfs:range xsd:string ;
          nrl:maxCardinality 1 .

    nbib:mapScale
          a       rdf:Property ;
          rdfs:domain nbib:Map ;
          rdfs:comment "The scale of a map" ;
          rdfs:label "Map Scale" ;
          rdfs:range xsd:string ;
          nrl:maxCardinality 1 .

    nbib:article
          a       rdf:Property ;
          rdfs:domain nbib:Collection ;
          rdfs:comment "Connects an article to its collection (article in Newspaper, Proceedings, Journalissue)" ;
          rdfs:label "article" ;
          rdfs:subPropertyOf nie:hasLogicalPart ;
          nrl:inverseProperty nbib:collection ;
          rdfs:range nbib:Article .

    nbib:referencedPart
          a       rdf:Property ;
          rdfs:domain nbib:Reference ;
          rdfs:comment "The specific part of the document of a reference. Used to reference a chapter or quote a small portion of a publication" ;
          rdfs:label "referencedChapter" ;
          rdfs:range nbib:DocumentPart ;
          rdfs:subPropertyOf nie:hasLogicalPart ;
          nrl:maxCardinality 1 .

    nbib:documentPart
          a       rdf:Property ;
          rdfs:domain nbib:Publication ;
          rdfs:comment "Connects a publication to a part of it (for example a chapter or quoted passage)" ;
          rdfs:label "documentPart" ;
          nrl:inverseProperty nbib:documentPartOf ;
          rdfs:range nbib:DocumentPart .

    nbib:documentPartOf
          a       rdf:Property ;
          rdfs:domain nbib:DocumentPart ;
          rdfs:comment "Connects a part of a document to the publication it is from" ;
          rdfs:label "documentPartOf" ;
          nrl:inverseProperty nbib:documentPart ;
          rdfs:range nbib:Publication ;
          nrl:maxCardinality 1 .

    nbib:reference
          a       rdf:Property ;
          rdfs:domain nbib:Publication ;
          rdfs:comment "All references of a publication. Used to quickly get all different references (different quotes, chapters etc)" ;
          rdfs:label "reference" ;
          nrl:inverseProperty nbib:publication ;
          rdfs:range nbib:Reference .

    nbib:citedReference
          a       rdf:Property ;
          rdfs:domain nie:InformationElement ;
          rdfs:comment "Links all cited references from one publication. Good way to find new sources to read" ;
          rdfs:label "cited reference" ;
          rdfs:range nbib:Reference .

    nbib:publication
          a       rdf:Property ;
          rdfs:domain nbib:Reference ;
          rdfs:comment "The publication used for this reference" ;
          rdfs:label "publication" ;
          nrl:inverseProperty nbib:reference ;
          rdfs:range nbib:Publication ;
          nrl:maxCardinality 1 .

    nbib:publicationMethod
          a       rdf:Property ;
          rdfs:domain nbib:Publication ;
          rdfs:comment "How it was published, if the publishing method is nonstandard." ;
          rdfs:label "publicationMethod" ;
          rdfs:range xsd:string ;
          nrl:maxCardinality 1 .

    nbib:isbn
          a       rdf:Property ;
          rdfs:domain nbib:Publication ;
          rdfs:comment "The International Standard Book Number." ;
          rdfs:label "ISBN" ;
          rdfs:range xsd:string ;
          rdfs:subPropertyOf nao:identifier ;
          nrl:maxCardinality 1 .

    nbib:issn
          a       rdf:Property ;
          rdfs:domain nbib:Series ;
          rdfs:comment "The International Standard Serial Number. Used to identify a series of publications." ;
          rdfs:label "ISSN" ;
          rdfs:range xsd:string ;
          rdfs:subPropertyOf nao:identifier ;
          nrl:maxCardinality 1 .

    nbib:collection
          a       rdf:Property ;
          rdfs:domain nbib:Article ;
          rdfs:comment "The collection this article was published in (for example a Journalissue, Newspaper or Proceedings" ;
          rdfs:label "collection" ;
          rdfs:range nbib:Collection ;
          nrl:inverseProperty nbib:article ;
          nrl:cardinality 1 ;
          nrl:maxCardinality 1 .

    nbib:lccn
          a       rdf:Property ;
          rdfs:domain nbib:Publication ;
          rdfs:comment "The Library of Congress Call Number." ;
          rdfs:label "LCCN" ;
          rdfs:range xsd:string ;
          rdfs:subPropertyOf nao:identifier ;
          nrl:maxCardinality 1 .

    nbib:mrNumber
          a       rdf:Property ;
          rdfs:domain nbib:Publication ;
          rdfs:comment "The Mathematical Reviews number." ;
          rdfs:label "MRNumber" ;
          rdfs:range xsd:string ;
          rdfs:subPropertyOf nao:identifier ;
          nrl:maxCardinality 1 .

    nbib:numberOfPages
          a       rdf:Property ;
          rdfs:domain nbib:Publication ;
          rdfs:comment "The number of pages contained in the publication." ;
          rdfs:label "number of pages" ;
          rdfs:range xsd:integer ;
          nrl:maxCardinality 1 .

    nbib:numberOfVolumes
          a       rdf:Property ;
          rdfs:domain nbib:Publication ;
          rdfs:comment "The number of volumes that exists for a publication." ;
          rdfs:label "number of volumes" ;
          rdfs:range xsd:integer ;
          nrl:maxCardinality 1 .

    nbib:number
          a       rdf:Property ;
          rdfs:domain nbib:Publication ;
          rdfs:comment "The '(issue) number' of a journal, magazine, or tech-report, pr the publicl aw Number of a Statute or the number of a patent etc" ;
          rdfs:label "Issue Number" ;
          rdfs:range xsd:string ;
          nrl:maxCardinality 1 .

    nbib:organization
          a       rdf:Property ;
          rdfs:domain nbib:Publication ;
          rdfs:comment "The organization that held the conference where the proceedings comes from or that is otherwise responsible for the publication" ;
          rdfs:label "Organization" ;
          rdfs:range nco:OrganizationContact ;
          nrl:inverseProperty nbib:conference ;
          nrl:maxCardinality 1 .

    nbib:event
          a       rdf:Property ;
          rdfs:domain nbib:Publication ;
          rdfs:comment "The event this publication was shown, represented, published etc" ;
          rdfs:label "Event" ;
          rdfs:range pimo:Event ;
          nrl:inverseProperty nbib:eventPublication ;
          nrl:maxCardinality 1 .

    nbib:eventPublication
          a       rdf:Property ;
          rdfs:domain pimo:Event ;
          rdfs:comment "the publications that fornm the result of an event" ;
          rdfs:label "Event Publications" ;
          nrl:inverseProperty nbib:event ;
          rdfs:range nbib:Publication .

    nbib:pages
          a       rdf:Property ;
          rdfs:domain nbib:Reference ;
          rdfs:comment "Page numbers, separated either by commas or double-hyphens." ;
          rdfs:label "Pages" ;
          rdfs:range xsd:string ;
          nrl:maxCardinality 1 .

    nbib:pageStart
          a       rdf:Property ;
          rdfs:domain nbib:Chapter ;
          rdfs:comment "Starting page number of the chapter" ;
          rdfs:label "starting page" ;
          rdfs:range xsd:integer ;
          nrl:maxCardinality 1 .

    nbib:pageEnd
          a       rdf:Property ;
          rdfs:domain nbib:Chapter ;
          rdfs:comment "Ending page number of the chapter" ;
          rdfs:label "ending page" ;
          rdfs:range xsd:integer ;
          nrl:maxCardinality 1 .

    nbib:applicationNumber
          a       rdf:Property ;
          rdfs:domain nbib:Patent ;
          rdfs:comment "The application number of a patent" ;
          rdfs:label "Application Number" ;
          rdfs:range xsd:string ;
          nrl:maxCardinality 1 .

    nbib:priorityNumbers
          a       rdf:Property ;
          rdfs:domain nbib:Patent ;
          rdfs:comment "The priority number of a patent" ;
          rdfs:label "Priority Number" ;
          rdfs:range xsd:string .

    nbib:publicLawNumber
          a       rdf:Property ;
          rdfs:domain nbib:Statute ;
          rdfs:comment "The public law number of the statute" ;
          rdfs:label "Public Law Number" ;
          rdfs:range xsd:string .

    nie:publicationDate
          a       rdf:Property ;
          rdfs:domain nie:InformationElement ;
          rdfs:comment "The date of the publication" ;
          rdfs:label "Publication Date" ;
          rdfs:range xsd:dateTime ;
          nrl:maxCardinality 1 .

    nbib:filingDate
          a       rdf:Property ;
          rdfs:domain nbib:Patent ;
          rdfs:comment "The date when the patent was filed, the issue date is the same as the publication date" ;
          rdfs:label "Filing Date" ;
          rdfs:range xsd:dateTime ;
          nrl:maxCardinality 1 .

    nbib:patentReferences
          a       rdf:Property ;
          rdfs:domain nbib:Patent ;
          rdfs:comment "The references for this patent" ;
          rdfs:label "Patent references" ;
          rdfs:range xsd:string .

    nbib:legalStatus
          a       rdf:Property ;
          rdfs:domain nbib:Patent ;
          rdfs:comment "The legal status of this patent" ;
          rdfs:label "Legal Status" ;
          rdfs:range xsd:string .

    nbib:arguedDate
          a       rdf:Property ;
          rdfs:domain nbib:LegalDocument ;
          rdfs:comment "The date on which a legal case is argued before a court." ;
          rdfs:label "date argued" ;
          rdfs:range xsd:dateTime ;
          nrl:maxCardinality 1 .

    nbib:pubMed
          a       rdf:Property ;
          rdfs:domain nbib:Publication ;
          rdfs:comment "The PubMed ID." ;
          rdfs:label "PubMed ID" ;
          rdfs:range xsd:string ;
          rdfs:subPropertyOf nao:identifier ;
          nrl:maxCardinality 1 .

    nbib:inSeries
          a       rdf:Property ;
          rdfs:domain nbib:Publication ;
          rdfs:comment "The series the publication was published in. (for example a series of books, a series of lecture notes, a journal series" ;
          rdfs:label "inSeries" ;
          rdfs:range nbib:Series ;
          rdfs:subPropertyOf nie:hasLogicalPart ;
          nrl:maxCardinality 1 .

    nbib:seriesOf
          a       rdf:Property ;
          rdfs:domain nbib:Series ;
          rdfs:comment "The publication this series belongs to" ;
          rdfs:label "seriesOf" ;
          rdfs:range nbib:Publication ;
          rdfs:subPropertyOf nie:hasLogicalPart .

    nbib:publicationType
          a       rdf:Property ;
          rdfs:domain nbib:Publication ;
          rdfs:comment "The type of tech-report or other kind of Publication, for example, 'Research Note'." ;
          rdfs:label "Publication Type" ;
          rdfs:range xsd:string ;
          nrl:maxCardinality 1 .

    nbib:shortTitle
          a       rdf:Property ;
          rdfs:domain nbib:Publication ;
          rdfs:comment "The short version of the title" ;
          rdfs:label "Short Title" ;
          rdfs:range xsd:string ;
          nrl:maxCardinality 1 .

    nbib:translationOf
          a       rdf:Property ;
          rdfs:domain nbib:Publication ;
          rdfs:comment "Relates a translated document to the original document." ;
          rdfs:label "translation of" ;
          rdfs:range nbib:Publication ;
          rdfs:subPropertyOf nie:isLogicalPartOf ;
          nrl:maxCardinality 1 .

    nbib:volume
          a       rdf:Property ;
          rdfs:domain nbib:Publication  ;
          rdfs:comment "The volume of a journal or multi-volume book." ;
          rdfs:label "Volume" ;
          rdfs:range xsd:string ;
          nrl:maxCardinality 1 .

}

<http://www.example.com/nbib_metadata#>
{<http://www.example.com/nbib_metadata#>
          a       nrl:GraphMetadata ;
          nrl:coreGraphMetadataFor
                  nbib: .

nbib:  a       nrl:Ontology ;
          nao:creator <Joerg.Ehrichs@gmx.de> ;
          nao:hasDefaultNamespace
                  "http://www.example.com/nbib#" ;
          nao:hasDefaultNamespaceAbbreviation
                  "nbib" ;
          nao:lastModified "2011-12-07T10:36:58Z" ;
          nao:status "Unstable" ;
          nao:updatable "0 " ;
          nao:version "0.1" ;
          nao:prefLabel "Sync NBIB Ontology" ;
          nao:description "Describes all necessary parts to keep the publication from NBIB insync with an online storage such as zotero" .

}

























